\documentclass{article}

\usepackage{amsmath}
\usepackage{tikz}

\begin{document}

\section{Gradient Descent}
\def\avgsum[#1,#2]{\frac{1}{#2}\sum_{#1=1}^{#2}}

\begin{align}
	C'(w) = \lim_{\epsilon \to 0}\frac{C(w + \epsilon) - C(w)}{\epsilon}
\end{align}

\subsection{``Double``}

\begin{align}
	C(w)  &= \avgsum[i,n](x_iw - y_i)^2 \\  
	C'(w) &= \left(\avgsum[i,n](x_iw - y_i)^2\right)' \\
		  &= \frac{1}{n}\left(\sum_{i=1}^{n}(x_iw - y_i)^2\right)' \\
		  &= \frac{1}{n}\left((x_0w - y_0)^2 + (x_1w - y_1)^2 + \hdots+(x_nw - y_n)^2\right)' \\
		  &= \avgsum[i,n]\left((x_iw - y_i)^2\right)' \\
		  &= \avgsum[i,n]2(x_iw - y_i)\left(x_iw - y_i\right)' \\
		  &= \avgsum[i,n]2(x_iw - y_i)\left(x_iw\right)' \\
		  &= \avgsum[i,n]2(x_iw - y_i)x_i' \\
\end{align}

\begin{align}
	C(w)  &= \avgsum[1,n](x_iw - y_i)^2 \\  
	C'(w) &= \avgsum[1,n]2(x_iw - y_i)x_i' \\
\end{align}

\subsection{One neuron model}

\def\d{1.5}

\begin{center}
	\begin{tikzpicture}
		\node (X) at (-\d, 0) {$x$};
		\node[shape=circle,draw=black] (N) at (0,0) {$\sigma, w, b$};
		\node at (\d, 0) (Y) {$y$};
		\path[->] (X) edge (N);
		\path[->] (N) edge (Y);
	\end{tikzpicture}
\end{center}

\begin{align}
	y &= \sigma(xw + b) \\
	\sigma(x) &= \frac{1}{1 + e^{-x}} \\
	\sigma'(x) &= \sigma(x)(1 - \sigma(x)) \\
\end{align}

\subsubsection{Cost}

\def\pd[#1]{\partial_{#1}}

\begin{align}
	a_i &= \sigma(x_iw + b) \\
	\pd[w]a_i 
		&= \pd[w]\left(\sigma(x_iw + b)\right) \\
		&= a_i(1 - a_i)\pd[w](x_iw + b) \\
		&= a_i(1 - a_i)x_i \\
	\pd[b]a_i 
		&= a_i(1 - a_i) \\
	C &= \avgsum[i,n](a_i - y_i)^2 \\
	\pd[w]C 
		&= \pd[w]\left(\avgsum[i,n](a_i - y_i)^2\right) \\
		&= \avgsum[i,n]\pd[w]\left((a_i - y_i)^2\right) \\
		&= \avgsum[i,n]2(a_i - y_i)\pd[w]\left(a_i - y_i\right) \\
		&= \avgsum[i,n]2(a_i - y_i)\pd[w]a_i \\
		&= \avgsum[i,n]2(a_i - y_i)(a_i(1 - a_i)x_i) \\
	\pd[b]C 
		&= \avgsum[i,n]2(a_i - y_i)\pd[b]a_i \\
		&= \avgsum[i,n]2(a_i - y_i)(a_i(1 - a_i)) \\
\end{align}

\subsection{One Neuron Model with 2 inputs}

\def\2d{2}

\begin{center}
	\begin{tikzpicture}
		\node (X) at (-\2d, 2) {$x$};
		\node (Y) at (-\2d, 0) {$y$};
		\node[shape=circle,draw=black] (N) at (0,1) {$\sigma, b$};
		\node at (\2d, 1) (Z) {$z$};
		\path[->] (X) edge node[above] {$w_1$} (N);
		\path[->] (Y) edge node[below] {$w_2$} (N);
		\path[->] (N) edge (Z);
	\end{tikzpicture}
\end{center}

\begin{align}
	z &= \sigma(x_iw_1 + y_iw_2 + b) \\
	\sigma(x) &= \frac{1}{1 + e^{-x}} \\
	\sigma'(x) &= \sigma(x)(1 - \sigma(x)) \\
\end{align}

\subsubsection{Cost}

\begin{align}
	a_i &= \sigma(x_iw_1 + y_iw_2 + b) \\
	\pd[w_1]a_i 
		&= \pd[w]\left(\sigma(x_iw_1 + y_iw_2 + b)\right) \\
		&= a_i(1 - a_i)\pd[w](x_iw_1 + y_iw_2 + b) \\
		&= a_i(1 - a_i)x_i \\
	\pd[w_2]a_i 
		&= a_i(1 - a_i)y_i \\
	\pd[b]a_i 
		&= a_i(1 - a_i) \\
	C &= \avgsum[i,n](a_i - z_i)^2 \\
	\pd[w_1]C 
		&= \pd[w_1]\left(\avgsum[i,n](a_i - z_i)^2\right) \\
		&= \avgsum[i,n]\pd[w_1]\left((a_i - z_i)^2\right) \\
		&= \avgsum[i,n]2(a_i - z_i)\pd[w_1]\left(a_i - z_i\right) \\
		&= \avgsum[i,n]2(a_i - z_i)\pd[w_1]a_i \\
		&= \avgsum[i,n]2(a_i - z_i)(a_i(1 - a_i)x_i) \\
	\pd[w_2]C 
		&= \avgsum[i,n]2(a_i - z_i)(a_i(1 - a_i)y_i) \\
	\pd[b]C 
		&= \avgsum[i,n]2(a_i - z_i)\pd[b]a_i \\
		&= \avgsum[i,n]2(a_i - z_i)(a_i(1 - a_i)) \\
\end{align}

\subsection{Two Neuron Model with 1 input}

\begin{center}
	\begin{tikzpicture}
		\node (X) at (-\d, 0) {$a^{(0)}$};
		\node[shape=circle,draw=black] (N1) at (0,0) {$\sigma, b^{(1)}$};
		\node[shape=circle,draw=black] (N2) at (1.5*\d,0) {$\sigma, b^{(2)}$};
		\node at (2.5*\d, 0) (Y) {$a^{(2)}$};
		\path[->] (X) edge node[above] {$w_1$} (N1);
		\path[->] (N1) edge node[above] {$w_2$} (N2);
		\path[->] (N2) edge (Y);
	\end{tikzpicture}
\end{center}

\begin{align}
	a^{(1)} &= \sigma\left(a^{(0)}w^{(1)} + b^{(1)}\right) \\	
	a^{(2)} &= \sigma\left(a^{(1)}w^{(2)} + b^{(2)}\right) \\
\end{align}

\subsubsection{Cost}

\begin{align}
	a_i^{(1)} &= \sigma\left(a_i^{(0)}w^{(1)} + b^{(1)}\right) \\	
	a_i^{(2)} &= \sigma\left(a_i^{(1)}w^{(2)} + b^{(2)}\right) \\
	\pd[w^{(2)}]a_i^{(2)} 
		&= \pd[w^{(2)}] \sigma\left(a_i^{(1)}w^{(2)} + b^{(2)}\right) \\	
		&= a_i^{(2)}(1 - a_i^{(2)}) \pd[w^{(2)}] \left(a_i^{(1)}w^{(2)} + b^{(2)}\right) \\	
		&= a_i^{(2)}(1 - a_i^{(2)}) a_i^{(1)} \\	
	\pd[b^{(2)}]a_i^{(2)} 
		&= a_i^{(2)}(1 - a_i^{(2)}) \\	
	\pd[a^{(1)}]a_i^{(2)} 
		&= a_i^{(2)}(1 - a_i^{(2)})w^{(2)} \\	
	C^(2) &= \avgsum[i, n] (a_i^{(2)} - y_i)^2 \\
	\pd[w^{(2)}]C^(2)  
		&= \avgsum[i, n] pd[w^{(2)}](a_i^{(2)} - y_i)^2 \\
		&= \avgsum[i, n] 2(a_i^{(2)} - y_i) \pd[w^{(2)}]a_i^{(2)} \\
		&= \avgsum[i, n] 2(a_i^{(2)} - y_i) a_i^{(2)}(1 - a_i^{(2)}) a_i^{(1)} \\
	\pd[b^{(2)}]C^(2)  
		&= \avgsum[i, n] 2(a_i^{(2)} - y_i) a_i^{(2)}(1 - a_i^{(2)}) \\
	\pd[a^{(1)}]C^(2)  
		&= \avgsum[i, n] 2(a_i^{(2)} - y_i) a_i^{(2)}(1 - a_i^{(2)}) w^{(2)} \\
	e_i &= a_i^{(1)} - \pd[a_i^{(1)}]C^{(2)} \\
	C^(1) &= \avgsum[i, n] (a_i^{(1)} - e_i)^2 \\
	\pd[w^{(1)}]C^(1)  
		&= \pd[w^{(1)}]\left(\avgsum[i, n] (a_i^{(1)} - e_i)^2\right) \\
		&= \avgsum[i, n] \pd[w^{(1)}]\left((a_i^{(1)} - e_i)^2\right) \\
		&= \avgsum[i, n] 2(a_i^{(1)} - e_i)\pd[w^{(1)}](a_i^{(1)} - e_i) \\
		&= \avgsum[i, n] 2(a_i^{(1)} - e_i)\pd[w^{(1)}]a_i^{(1)} \\
		&= \avgsum[i, n] 2(a_i^{(1)} - (a_i^{(1)} - \pd[a_i^{(1)}]C^{(2)}))\pd[w^{(1)}]a_i^{(1)} \\
		&= \avgsum[i, n] 2(a_i^{(1)} - a_i^{(1)} + \pd[a_i^{(1)}]C^{(2)})\pd[w^{(1)}]a_i^{(1)} \\
		&= \avgsum[i, n] 2(\pd[a_i^{(1)}]C^{(2)})\pd[w^{(1)}]a_i^{(1)} \\
	\pd[b^{(1)}]C^(1)  
		&= \\
\end{align}

\end{document}
